\documentclass[a4paper]{article}
\usepackage{settings}
\begin{document}
	
\section{Proprietà integrali}
$$
\int (f(x) +g(x)) dx = \int f(x) dx + \int g(x) dx \\
$$
$$
\int k f(x) dx = k \int f(x) dx
$$

\section{Tabella primitive}
TODO

\section{Integrazione di una funzione composta}
La formula generica è:
$$
\int^b_a g'(f(x))f'(x) dx = \Big [ g (f(x)) \Big ]^{b}_{a}
$$
deriva da
$$
f: I \rightarrow J , g: J \rightarrow \mathbb{R} ,\  f,g\ derivabili 
$$
$$
\int^b_a {d \over dx} (g \circ f)(x) = \int^b_a g'(f(x))f'(x) dx = \Big [ g (f(x)) \Big ]^{b}_{a}
$$
\subsection{Integrali notevoli di funzioni composte}
$$

- \int f'(x) [ f'(x) ]^\alpha dx = {[f(x)]^{\alpha +1} \over \alpha +1} \ con \ \alpha \neq -1

- \int {f'(x) \over f(x)} dx = \ln |{ f(x)}| \ \textbf{NB:} questo \ è\ il\ caso\ \alpha = -1 \ della\ prec.

- \int f'(x) \cos f(x) dx = \sin f(x)

- \int f'(x) \sin f(x) dx = - \cos f(x)

- \int f'(x) e^{f(x)} dx = e^{f(x)}

$$
\end{document}
